theories/VLSM/Core/Equivocation/MsgDepFixedSetEquivocation.v
@@ -172,8 +172,12 @@ Proof.
   eapply VLSM_incl_in_futures in Hfutures as Hpre_futures
   ; [| apply constraint_preloaded_free_incl].
   apply (VLSM_projection_in_futures (preloaded_component_projection IM i)) in Hpre_futures.
-  eapply message_dependencies_are_necessary, has_been_directly_observed_sent_received_iff
-    in Hproduce as [Hreceived| Hsent]; [..| done | typeclasses eauto]; cycle 1.
+  destruct Hproduce as ((pre_destination, im) & l & Hti).
+  eapply message_dependencies_are_necessary in Hti as Hobs; [| typeclasses eauto].
+  eapply ram_transition_preserves_message_dependencies_full_node_condition
+    in Hobs; [| done..].
+  eapply has_been_directly_observed_sent_received_iff
+    in Hobs as [Hreceived| Hsent]; [..| done]; cycle 1.
   + left; exists i; split; [done |].
     eapply in_futures_preserving_oracle_from_stepwise
     ; [apply has_been_sent_stepwise_from_trace | done | done].
@@ -181,7 +185,7 @@ Proof.
   + apply in_futures_valid_fst in Hfutures as Hdestination.
     specialize (received_component_received_previously IM Hdestination Hreceived)
       as (s_item_dm & [] & Ht & Hfutures_dm & <- & Hinput);
-      destruct l as (i, li); cbn in Hinput; subst input; cbn in *.
+      destruct l0 as (i, li); cbn in Hinput; subst input; cbn in *.
       apply input_valid_transition_in_futures in Ht as Hfutures_t; cbn in Hfutures_t
       ; destruct Ht as [(_ & _ & _ & Hc) _].
       eapply in_futures_preserves_strong_fixed_equivocation; [| apply Hc].
@@ -212,9 +216,13 @@ Proof.
     destruct Hemit as ((sX, iom) & (sub_i, li) & sX' & HtX).
     eapply (preloaded_composite_directly_observed_valid _ _ _ sX').
     + by eapply input_valid_transition_destination.
-    + exists sub_i. destruct_dec_sig sub_i i Hi Heqsub_i; subst.
-      eapply message_dependencies_are_necessary; [typeclasses eauto | | done].
-      exists (sX (dexist i Hi), iom), li.
+    + exists sub_i; destruct_dec_sig sub_i i Hi Heqsub_i; subst.
+      cut (input_valid_transition (pre_loaded_with_all_messages_vlsm (IM i))
+        li (sX (dexist i Hi), iom) (sX' (dexist i Hi), Some m)).
+      {
+        intro Hti; eapply has_been_directly_observed_step_update; [done |].
+        by right; unfold sub_IM in *; eapply message_dependencies_are_necessary.
+      }
       eapply (VLSM_projection_input_valid_transition (single_equivocator_projection s i Hi))
       ; [| done].
       unfold sub_label_element_project; cbn.
